
@prefix yasgui:  <https://matdata.eu/ns/yasgui#> .
@prefix dcterms: <http://purl.org/dc/terms/> .
@prefix prov:    <http://www.w3.org/ns/prov#> .
@prefix skos:    <http://www.w3.org/2004/02/skos/core#> .
@prefix spin:    <http://spinrdf.org/spin#> .
@prefix rdfs:    <http://www.w3.org/2000/01/rdf-schema#> .

yasgui:Workspace
  a rdfs:Class ;
  rdfs:label "YASGUI Workspace" ;
  rdfs:comment "A SKOS ConceptScheme representing a YASGUI workspace. May contain folders (yasgui:WorkspaceFolder) and/or managed queries directly." ;
  rdfs:subClassOf skos:ConceptScheme .

yasgui:WorkspaceFolder
  a rdfs:Class ;
  rdfs:label "YASGUI Workspace Folder" ;
  rdfs:comment "A SKOS Concept that belongs to a workspace scheme and organizes managed queries hierarchically." ;
  rdfs:subClassOf skos:Concept .

yasgui:ManagedQuery
  a rdfs:Class ;
  rdfs:label "Managed Query" ;
  rdfs:comment "A logical SPARQL query artifact. It is placed either in a workspace (root) or a workspace folder. Versions are separate entities." ;
  rdfs:subClassOf prov:Entity .

yasgui:ManagedQueryVersion
  a rdfs:Class ;
  rdfs:label "Managed Query Version" ;
  rdfs:comment "An immutable version of a SPARQL query, with author, timestamp, endpoints, and textual representation." ;
  rdfs:subClassOf prov:Entity , spin:Query .
